\documentclass[10pt]{extarticle}
\title{}
\author{Avinash Iyer}
\date{}
\usepackage[shortlabels]{enumitem}


%paper setup
\usepackage{geometry}
\geometry{letterpaper, portrait, margin=1in}
\usepackage{fancyhdr}

%symbols
\usepackage{amsmath}
\usepackage{amssymb}
\usepackage{amsthm}
\usepackage{mathtools}
\usepackage{hyperref}
\usepackage{gensymb}
\usepackage{multirow,array}

\newtheorem*{remark}{Remark}
\usepackage[T1]{fontenc}
\usepackage[utf8]{inputenc}

%chemistry stuff
%\usepackage[version=4]{mhchem}
%\usepackage{chemfig}

%plotting
\usepackage{pgfplots}
\usepackage{tikz}
\tikzset{middleweight/.style={pos = 0.5, fill=white}}
\tikzset{weight/.style={pos = 0.5, fill = white}}
\tikzset{lateweight/.style={pos = 0.75, fill = white}}
\tikzset{earlyweight/.style={pos = 0.25, fill=white}}

%\usepackage{natbib}

%graphics stuff
\usepackage{graphicx}
\graphicspath{ {./images/} }
\usepackage[style=numeric, backend=biber]{biblatex} % Use the numeric style for Vancouver
\addbibresource{the_bibliography.bib}
%code stuff
%when using minted, make sure to add the -shell-escape flag
%you can use lstlisting if you don't want to use minted
%\usepackage{minted}
%\usemintedstyle{pastie}
%\newminted[javacode]{java}{frame=lines,framesep=2mm,linenos=true,fontsize=\footnotesize,tabsize=3,autogobble,}
%\newminted[cppcode]{cpp}{frame=lines,framesep=2mm,linenos=true,fontsize=\footnotesize,tabsize=3,autogobble,}

%\usepackage{listings}
%\usepackage{color}
%\definecolor{dkgreen}{rgb}{0,0.6,0}
%\definecolor{gray}{rgb}{0.5,0.5,0.5}
%\definecolor{mauve}{rgb}{0.58,0,0.82}
%
%\lstset{frame=tb,
%	language=Java,
%	aboveskip=3mm,
%	belowskip=3mm,
%	showstringspaces=false,
%	columns=flexible,
%	basicstyle={\small\ttfamily},
%	numbers=none,
%	numberstyle=\tiny\color{gray},
%	keywordstyle=\color{blue},
%	commentstyle=\color{dkgreen},
%	stringstyle=\color{mauve},
%	breaklines=true,
%	breakatwhitespace=true,
%	tabsize=3
%}
% text + color boxes
\usepackage[most]{tcolorbox}
\tcbuselibrary{breakable}
\newtcolorbox{problem}[1]{colback = white, title = {#1}, breakable}
\newtcolorbox{solution}{colback = white, colframe = black!75!white, title = Solution, breakable}
%including PDFs
%\usepackage{pdfpages}
\setlength{\parindent}{0pt}
\usepackage{cancel}
\pagestyle{fancy}
\fancyhf{}
\rhead{Avinash Iyer}
\lhead{Math 212: Homework 4}
\newcommand{\card}{\text{card}}
\newcommand{\ran}{\text{ran}}
\newcommand{\N}{\mathbb{N}}
\newcommand{\Q}{\mathbb{Q}}
\newcommand{\Z}{\mathbb{Z}}
\newcommand{\R}{\mathbb{R}}
\begin{document}
  \renewcommand{\arraystretch}{1.5}
  \begin{problem}{14.2}
    \begin{description}[font=\normalfont]
      \item[2:] \hfill
        \begin{align*}
          \nabla Q &= \begin{pmatrix}50\\100\end{pmatrix}
        \end{align*}
      \item[8:] \hfill
        \begin{align*}
          \nabla f &= \begin{pmatrix}0.3\left(\frac{L}{K}\right)^{0.7}\\ 0.7\left(\frac{K}{L}\right)^{0.3}\end{pmatrix}
        \end{align*}
      \item[14:]
        \begin{align*}
          \nabla z &= \begin{pmatrix}\frac{e^y}{x+y}-\frac{xe^y}{(x+y)^2}\\\frac{xe^y}{x+y}-\frac{xe^y}{(x+y)^2}\end{pmatrix}
        \end{align*}
      \item[22:]
        \begin{align*}
          \nabla f(0,1) &= \begin{pmatrix}\frac{1}{2}\\\frac{1}{2}\end{pmatrix}
        \end{align*}
      \item[32:] Approximately zero.
      \item[38:] $\hat i$
      \item[42:] $\hat i - \hat j$
      \item[44:] $\frac{5}{2\sqrt{2}}$
      \item[48:]
        \begin{align*}
          \nabla f(1,2) \cdot \vec u &= \begin{pmatrix}\frac{6}{5}\\-\frac{4}{5}\end{pmatrix}
        \end{align*}
      \item[50:] $\partial f = y\partial x + x\partial y$
    \end{description}
  \end{problem}
  \begin{problem}{14.3}
    \begin{description}[font=\normalfont]
      \item[2:]
        \begin{align*}
          \nabla f &= \begin{pmatrix}2x\\0\\0\end{pmatrix}
        \end{align*}
      \item[8:]
        \begin{align*}
          \nabla f &= \begin{pmatrix}e^y\sin z \\ xe^y\sin z \\ xe^y \cos z\end{pmatrix}
        \end{align*}
      \item[10:]
        \begin{align*}
          \nabla f &= \begin{pmatrix}2x_1x_2^3x_3^4 \\ 3x_1^2x_2^2x_3^4 \\ 4x_1^2x_2^3x_3^3\end{pmatrix}
        \end{align*}
      \item[14:]
        \begin{align*}
          \nabla f (1,1,1) &= \begin{pmatrix}2\\3\\4\end{pmatrix}
        \end{align*}
      \item[16:]
        \begin{align*}
          \nabla f (1,1,1) &= \begin{pmatrix}6\\3\\2\end{pmatrix}
        \end{align*}
      \item[18:]
        \begin{align*}
          \nabla f(2,1,e) &= \begin{pmatrix}1\\ \frac{2}{e} \\ \frac{2}{e}\end{pmatrix}
        \end{align*}
      \item[22:]
        \begin{align*}
          \nabla f \cdot \vec{u} &= 1
        \end{align*}
      \item[28:]
        \begin{align*}
          \shortintertext{Verifying Point on Level Surface:}
          (-1)^2 - (-1)(1)(2) &= 3\\
          \shortintertext{Finding Gradient:}
          f(x,y,z) &= x^2 - xyz\\
          \nabla f &= \begin{pmatrix}2x - yz \\ -xz \\ -xy\end{pmatrix}\\
          \nabla f (-1,1,2) &= \begin{pmatrix}-4\\2\\1\end{pmatrix}\\
          \shortintertext{Tangent Plane:}
          0 &= -4(x+1) + 2(y-1) + 1(z - 2) 
        \end{align*}
      \item[30:]
        \begin{align*}
          \shortintertext{Verifying Point on Level Surface:}
          1 &= \frac{4}{2(-1) + 3(2)}
          \shortintertext{Finding Gradient:}
          f(x,y,z) &= \frac{4}{y(2x + 3z)}\\
          \nabla f &= \begin{pmatrix}-\frac{8}{y(2x+3z)^2}\\-\frac{4}{y^2(2x + 3z)}\\ -\frac{12}{y(2x + 3z)^2}\end{pmatrix}\\
          \nabla f (-1,1,2) &= \begin{pmatrix}-\frac{1}{2} \\ -1 \\ -\frac{3}{4}\end{pmatrix}\\
          \shortintertext{Tangent Plane:}
          0 &= -\frac{1}{2}(x+1) -(y-1) -\frac{3}{4}(z - 2) 
        \end{align*}
    \end{description}
  \end{problem}
  \begin{problem}{14.4}
    \begin{description}[font=\normalfont]
      \item[2:]
        \begin{align*}
          \frac{dz}{dt} &= \sin^2 t + 2\sin t e^{-t}
        \end{align*}
      \item[10:]
        \begin{align*}
          \frac{\partial z}{\partial u} &= \frac{e^v}{u}\\
          \frac{\partial z}{\partial v} &= 2e^v + \frac{e^v}{u}
        \end{align*}
      \item[16:]
        \begin{align*}
          \frac{dz}{dt} &= \frac{\partial z}{\partial x}\frac{dx}{dt} + \frac{\partial z}{\partial y}\frac{dy}{dt}\\
                        &= 3t^{10} + 2t^{11}
        \end{align*}
      \item[18:]
        \begin{align*}
          \frac{dz}{dt}\biggr\vert_{t=1} &= \frac{\partial z}{\partial x}\frac{dx}{dt} + \frac{\partial z}{\partial y}\frac{dy}{dt}\\
                                         &= 802.2
        \end{align*}
      \item[20:]
        \begin{align*}
          \frac{dV}{dt} &= \frac{\partial V}{\partial R}\frac{dR}{dt} + \frac{\partial V}{\partial I}\frac{d I}{dt}\\
                        &= \frac{\partial V}{\partial R}\left(\frac{\partial R}{\partial R_1}\frac{dR_1}{dt} + \frac{\partial R}{\partial R_2}\frac{dR_2}{dt}\right) + \frac{\partial V}{\partial I}\frac{dI}{dt}\\
                        &= \frac{61}{160}
        \end{align*}
      \item[30:]
        \begin{align*}
          \frac{dh}{dt} &= \frac{\partial h}{\partial f}\frac{df}{dt} + \frac{\partial h}{\partial g}\frac{dg}{dt}\\
                        &= f'(t)g(t) + g'(t)f(t)
        \end{align*}
      \item[32:] I don't know how to do this problem.
      \item[34:]
        \begin{align*}
          \frac{\partial z}{\partial v} &= \frac{\partial z}{\partial x}\frac{\partial x}{\partial v} + \frac{\partial z}{\partial y}\frac{\partial y}{\partial v}\\
                                        &= bk + dq
        \end{align*}
    \end{description}
  \end{problem}
  \begin{problem}{14.5}
    \begin{description}[font=\normalfont]
      \item[6:]
        \begin{align*}
          \frac{\partial^2 f}{\partial x^2} &= 0\\
          \frac{\partial^2 f}{\partial y^2} &= xe^y\\
          \frac{\partial^2f}{\partial x \partial y} &= e^y\\
          \frac{\partial^2 f}{\partial y \partial x} &= e^y
        \end{align*}
      \item[10:]
        \begin{align*}
          \frac{\partial^2 f}{\partial x^2} &= -2\sin(x^2 + y^2) + 2\cos(x^2 + y^2)\\
          \frac{\partial^2 f}{\partial y^2} &= -2\sin(x^2 + y^2) + 2\cos(x^2 + y^2)\\
          \frac{\partial^2 f}{\partial x \partial y} &= -4xy\sin(x^2 + y^2)\\
          \frac{\partial^2 f}{\partial x \partial y} &= -4xy\sin(x^2 + y^2)
        \end{align*}
      \item[16:]
        \begin{align*}
          f(x,y) &\approx 1 -2x + y + 8x^2 + 2y^2 -4xy
        \end{align*}
      \item[20:] 
        \begin{align*}
        g(x,y) \approx x-2y -x^2 -4y^2 + 2xy
        \end{align*}
      \item[22:]
        \begin{enumerate}[(a)]
          \item $f_x(P) < 0$
          \item $f_y(P) = 0$
          \item $f_{xx}(P) > 0$
          \item $f_{yy}(P) = 0$
          \item $f_{xy}(P) = 0$
        \end{enumerate}
      \item[24:]
        \begin{enumerate}[(a)]
          \item $f_x(P) > 0$
          \item $f_y(P) = 0$
          \item $f_{xx}(P) < 0$
          \item $f_{yy}(P) = 0$
          \item $f_{xy}(P) = 0$
        \end{enumerate}
    \end{description}
  \end{problem}
\end{document}
