\documentclass[8pt]{mypackage}

% sans serif font:
%\usepackage{cmbright}
%\usepackage{sfmath}
%\usepackage{bbold} %better blackboard bold

%serif font + different blackboard bold for serif font
\usepackage{newpxtext,eulerpx}
\usepackage{eucal}
\renewcommand*{\mathbb}[1]{\varmathbb{#1}}
\renewcommand*{\hbar}{\hslash}

\pagestyle{fancy} %better headers
\fancyhf{}
\rhead{Avinash Iyer}
\lhead{Ordinary Differential Equations: Homework 12}

\setcounter{secnumdepth}{0}

\begin{document}
\RaggedRight
\section{Part 1}%
\subsection{3.6, Problem 3}%
We define $x_1= y$ and $x_2 = \diff{y}{t}$. We get
\begin{align*}
  \diff{x_1}{t} &= x_2\\
  \diff{x_2}{t} &= -9x_1 - 6x_2\\
  \diff{\vec{X}}{t} &= \begin{pmatrix}0 & 1 \\ -9 & -6\end{pmatrix} \vec{X}\\
  \det \begin{pmatrix}-\lambda & 1 \\ -9 & -6-\lambda\end{pmatrix} &= \lambda\left(\lambda + 6\right) + 9\\
  \lambda_1 &= -3\\
  \vec{v}_1 &= \begin{pmatrix}1\\-3\end{pmatrix}\\
  \vec{X}(t) &= e^{3t} \begin{pmatrix}s_0\\t_0\end{pmatrix} + te^{3t} \begin{pmatrix}3s_0 + t_0\\-9s_0-t_0\end{pmatrix}\\
  y(t) &= s_0e^{3t} + \left(3s_0 + t_0\right)te^{3t}.
\end{align*}
\subsection{3.6, Problem 4}%
Using the lucky guess, we let $y(t) = e^{st}$, yielding
\begin{align*}
  e^{st}\left(s^2 - 4s + 4\right) &= 0\\
  s &= 2\\
  y(t) &= k_1e^{2t} + k_2te^{2t}
\end{align*}
\subsection{3.6, Problem 11}%
Using the lucky guess method, we find the general solution of the form
\begin{align*}
  y(t) &= k_1e^{4t} + k_2te^{4t}.
\end{align*}
Finding $y(0)$, we get $k_1 = 3$. Taking derivatives, we then get
\begin{align*}
  11 &= 4k_1 + k_2,
\end{align*}
yielding $k_2 = -1$. The solution to the IVP is, then,
\begin{align*}
  y(t) &= 3e^{4t} - te^{4t}.
\end{align*}
\subsection{3.6, Problem 12}%
Using the lucky guess method, we find the general solution of the form
\begin{align*}
  y(t) &= k_1e^{2t} + k_2te^{2t}.
\end{align*}
Finding $y(0)$, we get $k_1 = 1$, and
\begin{align*}
  1 &= 2k_1 + k_2\\
  k_2 &= -1.
\end{align*}
The solution to the IVP is, then,
\begin{align*}
  y(t) &= e^{2t} - te^{2t}.
\end{align*}

\subsection{3.6, Problem 31}%
We have
\begin{align*}
  \diff{^2y}{t^2} + p\diff{y}{t} + qy &= 0\\
  \diff{^2}{t^2}\left(\re\left(y(t)\right) + i\im\left(y(t)\right)\right) + p\diff{}{t}\left(\re\left(y(t)\right) + i\im\left(y(t)\right)\right) + q\left(\re\left(y(t)\right) + i\im\left(y(t)\right)\right) &= 0\\
  \underbrace{\diff{^2}{t^2}\left(\re\left(y(t)\right)\right) + p\diff{}{t}\left(\re\left(y(t)\right)\right) + q\re\left(y(t)\right)}_{\text{Real}} + i\underbrace{\left(\diff{^2}{t^2}\left(\im\left(y(t)\right)\right) + p\diff{}{t}\left(\im\left(y(t)\right)\right) + q\im\left(y(t)\right)\right)}_{\text{Imaginary}} &= 0,
\end{align*}
meaning that both the Real and Imaginary portions must be equal to zero.\newline

Thus, both $\re\left(y(t)\right)$ and $\im\left(y(t)\right)$ are solutions.
\subsection{6.1, Problem 3}%
\begin{align*}
  \mathcal{L}\left[h\right] &= \int_{0}^{\infty} \left(-5t^2\right)e^{-st}\:dt\\
                            &= -5\int_{0}^{\infty} t^2e^{-st}\:dt\\
                            &= -5\left(-\frac{t^2}{s}e^{-st}\Bigr\vert_{0}^{\infty} - \frac{2t}{s^2}e^{-st}\Bigr\vert_{0}^{\infty} - \frac{2}{s^3}e^{-st}\Bigr\vert_{0}^{\infty}\right)\\
                            &= -\frac{10}{s^3}
\end{align*}
\subsection{6.1, Problem 4}%
\begin{align*}
  \mathcal{L}\left[k\right] &= \int_{0}^{\infty} t^5e^{-st}\:dt\\
                            &= \left(-\frac{t^5}{s}e^{-st} - \frac{5t^4}{s^2}e^{-st} - \frac{20t^3}{s^3}e^{-st} - \frac{60t^2}{s^4}e^{-st} - \frac{120t}{s^5}e^{-st} - \frac{120}{s^6}e^{-st}\right)\Bigr\vert_{0}^{\infty}\\
                            &= \frac{120}{s^{6}}
\end{align*}

\subsection{6.1, Problem 6}%
\begin{align*}
  \mathcal{L}\left[p\right] &= \sum_{k=0}^{n}a_k\mathcal{L}\left[t^k\right]\\
                            &= \sum_{k=0}^{n}\frac{a_k k!}{s^{k+1}}.
\end{align*}

\end{document}
