\documentclass[10pt]{mypackage}

% sans serif font:
%\usepackage{cmbright}
%\usepackage{sfmath}
%\usepackage{bbold} %better blackboard bold

%serif font + different blackboard bold for serif font
\usepackage{newpxtext,eulerpx}
\renewcommand*{\mathbb}[1]{\varmathbb{#1}}
\renewcommand*{\hbar}{\hslash}

\pagestyle{fancy} %better headers
\fancyhf{}
\rhead{Avinash Iyer}
\lhead{Ordinary Differential Equations: Homework 6}

\setcounter{secnumdepth}{0}

\begin{document}
\RaggedRight
\section{Part 1}%
\subsection{1.9, Problem 22}%
\begin{enumerate}[(a)]
  \item 
    \begin{align*}
      \diff{y}{t} - a(t)y = b(t)\\
      \mu(t)\diff{y}{t}-\mu(t)a(t)y &= \mu(t)b(t)\\
      e^{-\int_{0}^{t}\alpha(\tau)d\tau}\diff{y}{t}-e^{-\int_{0}^{t}\alpha(\tau)d\tau} &= e^{-\int_{0}^{t}\alpha(\tau)d\tau}b(t)\\
      \diff{}{t}\left(-\alpha(t)e^{-\int_{0}^{t}\alpha(\tau)d\tau}y\right) &= e^{-\int_{0}^{t}\alpha(\tau)d\tau}b(t).
    \end{align*}
  \item 
    \begin{align*}
      \diff{}{t}\left(\frac{1}{\mu(t)}\right) &= \diff{}{t}\left(e^{\int_{0}^{t}\alpha(\tau)d\tau}\right)\\
                                              &= \alpha(t)e^{\int_{0}^{t}\alpha(\tau)d\tau}\\
                                              &= \alpha(t)\left(\frac{1}{\mu(t)}\right).
    \end{align*}
  \item 
    \begin{align*}
      \diff{y_p}{t} &= \diff{}{t}\left(\frac{1}{\mu(t)}\right)\int_{0}^{t} \mu(\tau)b(\tau)\:d\tau + \frac{1}{\mu(t)}\diff{}{t}\left(\int_{0}^{t} \mu(\tau)b(\tau)\:d\tau\right)\\
                    &= \alpha(t)\left(\frac{1}{\mu(t)}\int_{0}^{t} \mu(\tau)b(\tau)\:d\tau\right) + b(t)\\
                    &= \alpha(t)y_p(t) + b(t).
    \end{align*}
  \item The general solution is, thus,
    \begin{align*}
      y(t) &= \frac{1}{\mu(t)}\int_{0}^{t} \mu(\tau)b(\tau)\:d\tau + C\frac{1}{\mu(t)}.
    \end{align*}
  \item These results are very similar to the case of 
    \begin{align*}
      y(t) &= \frac{1}{\mu(t)}\int_{}^{} \mu(t)b(t)\:dt,
    \end{align*}
    but instead of the indefinite integral, we use the equivalent expression using the definite integral.
  \item 
    \begin{align*}
      \mu(t) &= e^{-\int_{0}^{t}a(\tau)d\tau}\\
             &= e^{t^2}\\
      y(t) &= e^{-t^2}\int_{0}^{t} e^{\tau^2}\left(4e^{-\tau^2}\right)\:d\tau + Ce^{-t^2}\\
           &= 4te^{-t^2} + Ce^{-t^2}.
    \end{align*}
\end{enumerate}
\subsection{1.9, Problem 24}%
\begin{align*}
  \diff{S}{t} &= 2 - \frac{S}{15 + t}\\
  \diff{S}{t} + \frac{S}{15+t} &= 2\\
  \diff{}{t}\left((15+t)S\right) &= 2\left(15 + t\right)\\
  S &= \frac{30t + t^2}{15+t} + \frac{C}{15+t}\\
  S(0) &= \frac{C}{15}\\
       &= 6\\
  C &= 90\\
  S &= \frac{30t + t^2}{15+t} + \frac{90}{15+t}\\
  S(15) &= 25.5
\end{align*}
\end{document}
