\documentclass[10pt]{mypackage}

% sans serif font:
%\usepackage{cmbright}
%\usepackage{sfmath}
%\usepackage{bbold} %better blackboard bold

%serif font + different blackboard bold for serif font
\usepackage{newpxtext,eulerpx}
\renewcommand*{\mathbb}[1]{\varmathbb{#1}}
\renewcommand*{\hbar}{\hslash}

\pagestyle{fancy} %better headers
\fancyhf{}
\rhead{Avinash Iyer}
\lhead{Ordinary Differential Equations: Homework 5}

\setcounter{secnumdepth}{0}

\begin{document}
\RaggedRight
\section{Part 1}%
\subsection{1.8, Problem 4}%
To solve
\begin{align*}
  \diff{y}{t} &= 2y + \sin 2t,
\end{align*}
we start by solving the homogeneous equation
\begin{align*}
  \diff{y}{t} &= 2y,
\end{align*}
which yields $y_{h} = ke^{2t}$.\newline

For the particular solution, we guess that $y$ is of the form
\begin{align*}
  y_p(t) &= A\cos 2t + B\sin 2t.
\end{align*}
Plugging this into our equation, we get
\begin{align*}
  -2A\sin 2t + 2B\cos 2t + 2\left(A\cos 2t + B\sin 2t\right) &= \sin 2t\\
  \left(2B - 2A\right) \sin 2t + \left(2B + 2A\right)\cos 2t &= \sin 2t,
\end{align*}
meaning $A = -\frac{1}{4}$ and $B = \frac{1}{4}$. Thus, our general solution is
\begin{align*}
  y(t) &= -\frac{1}{4}\cos 2t + \frac{1}{4}\sin 2t + ke^{2t}.
\end{align*}
\subsection{1.8, Problem 8}%
To solve
\begin{align*}
  \diff{y}{t}-2y &= 3e^{-2t},
\end{align*}
with the initial condition of $y(0) = 10$, we start by solving the homogeneous equation, which yields $y_h(t) = ke^{2t}$.\newline

For the particular solution, we guess that $y$ is of the form
\begin{align*}
  y_p(t) &= Ae^{-2t}.
\end{align*}
Substituting into our equation, we have
\begin{align*}
  -2Ae^{-2t} - 2\left(Ae^{-2t}\right) &= 3e^{-2t}\\
  -4Ae^{-2t} &= 3e^{-2t},
\end{align*}
which yields $A = -\frac{3}{4}$. Thus, our general solution is of the form
\begin{align*}
  y(t) &= -\frac{3}{4}e^{-2t} + ke^{2t}.
\end{align*}
The initial condition yields $k = \frac{43}{4}$.
\subsection{1.8, Problem 9}%
To solve
\begin{align*}
  \diff{y}{t} + y &= \cos 2t,
\end{align*}
with the initial condition of $y(0) = 5$, we start by solving the homogeneous equation, which yields $y_h(t) = ke^{-t}$.\newline

For the particular solution, we guess that $y$ is of the form
\begin{align*}
  y_p(t) &= A\cos 2t + B\sin 2t.
\end{align*}
Substituting into our equation, we get
\begin{align*}
  -2A\sin 2t + 2B\cos 2t + \left(A\cos 2t + B\sin 2t\right) &= \cos 2t\\
  \left(2B + A\right)\cos 2t + \left(B - 2A\right)\sin 2t &= \cos 2t,
\end{align*}
meaning $A = \frac{1}{3}$ and $B = \frac{2}{3}$. Thus, our general solution is
\begin{align*}
  y(t) &= \frac{1}{3}\cos 2t + \frac{2}{3}\sin 2t + ke^{-t}.
\end{align*}
Solving the initial condition yields $k = \frac{14}{3}$.
\subsection{1.8, Problem 17}%
\begin{enumerate}[(a)]
  \item 
    \begin{align*}
      \frac{d}{dt}\left(\frac{1}{1-t}\right) &= \frac{1}{\left(1-t\right)^2}\\
                                             &= \left(\frac{1}{1-t}\right)^2.
    \end{align*}
  \item 
    \begin{align*}
      \diff{}{t}\left(\frac{2}{1-t}\right) &= \frac{2}{\left(1-t\right)^2}\\
                                           &\neq \left(\frac{2}{1-t}\right)^2.
    \end{align*}
  \item These two facts do not contradict the linearity principle since the equation $\diff{y}{t} = y^2$ is not a linear equation.
\end{enumerate}
\subsection{1.8, Problem 18}%
\begin{enumerate}[(a)]
  \item The solution of $y(t) = 2$ is an equilibrium solution for this equation.
  \item 
    \begin{align*}
      \diff{}{t}\left(2-e^{-t}\right) &= e^{-t}\\
                                      &= 2 - \left(2-e^{-t}\right)\\
                                      &= 2-y.
    \end{align*}
  \item The uniqueness of solutions implies that the only initial solution to an IVP with $y(0) = a$ for $a\neq 2$ is one that satisfies $y(t) = 2-e^{-t}$, which is not able to be added or multiplied by a constant.
\end{enumerate}
\subsection{1.8, Problem 20}%
\begin{align*}
  \left(2at + b\right) + 2\left(at^2 + bt + c\right) &= 3t^2 + 2t - 1\\
  2at^2 + \left(2a + 2b\right)t + \left(b+c\right) &= 3t^2 + 2t - 1.
\end{align*}
Thus, $a = \frac{3}{2}$, $b = -\frac{1}{2}$, and $c = -\frac{1}{2}$.
\subsection{1.8, Problem 31}%
To represent the first 30 years, we get
\begin{align*}
  \diff{y}{t} &= 5000 + 0.07y
\end{align*}
Solving the initial value problem with $y(0) = 0$, we get
\begin{align*}
  y(t) &= \frac{5000}{0.07}e^{0.07t} - \frac{5000}{0.07}.
\end{align*}
Then, $y(30) = 511869$.\newline

Now, using a different initial value problem, we solve
\begin{align*}
  \diff{y}{t} &= -36000 + 0.07y
\end{align*}
under the initial value of $y(0) = 511869$. Thus, we get
\begin{align*}
  y(t) &= Ke^{0.07t} + \frac{36000}{0.07}.
\end{align*}
Solving for $K$, we get $K = -2416.43$. Thus,
\begin{align*}
  t &= \frac{1}{0.07}\left(\ln\frac{36000}{(0.07)(2416.43)}\right)\\
    &= 76.
\end{align*}
\subsection{1.9, Problem 4}%
\begin{align*}
  \diff{y}{t} &= -2ty + 4e^{-t^2}\\
  \diff{y}{t} + 2ty &= 4e^{-t^2}\\
  e^{t^2}\diff{y}{t} + 2te^{t^2}y &= 4e^{-t^2}e^{t^2}\\
  \diff{}{t}\left(e^{t^2}y\right) &= 4\\
  e^{t^2}y &= 4t + C\\
  y &= \frac{4t}{e^{t^2}} + Ce^{-t^2}.
\end{align*}
\subsection{1.9, Problem 5}%
\begin{align*}
  \diff{y}{t} - \frac{2t}{1 + t^2}y &= 3\\
  \frac{1}{1 + t^2}\diff{y}{t} - \frac{2t}{1 + t^2}y &= \frac{3}{1 + t^2}\\
  \diff{}{t}\left(y\frac{1}{1+t^2}\right) &= \frac{3}{1+t^2}\\
  y\frac{1}{1+t^2} &= 3\arctan(t) + C\\
  y &= 3\arctan(t)\left(1+t^2\right) + C\left(1 + t^2\right).
\end{align*}
\subsection{1.9, Problem 9}%
\begin{align*}
  \diff{y}{t} &= -\frac{y}{t} + 2\\
  \diff{y}{t} + \frac{y}{t} &= 2\\
  t\diff{y}{t} + y &= 2t\\
  \diff{}{t}\left(ty\right) &= 2t\\
  ty &= t^2 + C\\
  y &= t + \frac{C}{t}.\\
  y(1) &= 1 + \frac{C}{1}\\
       &= 3\\
  C &= 2\\
  y(t) &= t + \frac{2}{t}.
\end{align*}
\subsection{1.9, Problem 12}%
\begin{align*}
  \diff{y}{t} - \frac{3}{t}y &= 2t^3e^{2t}\\
  \frac{1}{t^3}\diff{y}{t} - \frac{3}{t^4}y &= 2e^{2t}\\
  \diff{}{t}\left(\frac{1}{t^3}y\right) &= 2e^{2t}\\
  \frac{1}{t^3}y &= e^{2t} + C\\
  y &= t^3e^{2t} + Ct^3.\\
  y(1) &= 1 + C\\
      &= 0\\
  C &= -1\\
  y(t) &= t^3e^{2t} - t^3.
\end{align*}
\subsection{1.9, Problem 19}%
The only value of $a$ for which there is an explicit solution to the differential equation $\diff{y}{t} = aty + 4e^{-t^2}$ is with $a = t$.
\subsection{1.9, Problem 21}%
\begin{enumerate}[(a)]
  \item 
    \begin{align*}
      \diff{v}{t} + 0.4v &= 3\cos(2t)\\
      e^{0.4t}\diff{v}{t} + 0.4e^{0.4t}v &= 3e^{0.4t}\cos(2t)\\
      \diff{}{t}\left(e^{0.4t}v\right) &= 3e^{0.4t}\cos(2t)\\
      e^{0.4t}v &= \frac{3}{\left(\frac{\left(0.4\right)^2}{4}+1\right)}e^{0.4t}\left(\frac{1}{2}\sin(2t) + \frac{1}{4}\cos(2t)\right) + C\\
      v &= \frac{3}{\left(\frac{\left(0.4\right)^2}{4}+1\right)}\left(\frac{1}{2}\sin(2t) + \frac{1}{4}\cos(2t)\right) + \frac{C}{e^{0.4t}}.
    \end{align*}
  \item The homogeneous equation $\diff{v}{t} = -0.04v$ is solved by $v_h(t) = e^{-0.4t}$.\newline

    For the particular solution, we will use the guess that $v = A\cos 2t + B\sin 2t$. Then,
    \begin{align*}
      -A\sin 2t + B\cos 2t + 0.4\left(A\cos 2t + B\sin 2t\right) &= 3\cos 2t\\
      \left(0.4A + B\right)\cos 2t + \left(0.4B - A\right)\sin 2t &= 3\cos 2t,
    \end{align*}
    meaning $A = 0.4 B$, $1.4B = 3$, so $B = \frac{3}{1.4}$ and $A = 0.4\frac{3}{1.4}$. Thus, the general solution is
    \begin{align*}
      y(t) &= \frac{3}{1.4}\sin 2t + \frac{(0.4)(3)}{1.4}\cos 2t + C e^{-0.4}t.
    \end{align*}
\end{enumerate}
The latter method was quite a bit easier than the former method.
\end{document}
